src/program_proof/tulip/program/txn/proph.v
@@ -11,7 +11,20 @@ Section proph.
       ResolveRead #p #tid #(LitString key) @ ∅
     <<< ∃ acs', ⌜acs = ActRead ts key :: acs'⌝ ∗ own_txn_proph p acs' >>>
     {{{ RET #(); True }}}.
-  Admitted.
+  Proof.
+    iIntros "!> %Φ %Hts AU". wp_rec. wp_pures.
+    replace (⊤ ∖ ∅) with (⊤ : coPset) by set_solver.
+    iMod "AU" as (acs) "[(%pvs & %Hpvs & Hp) Hclose]".
+    wp_apply (wp_resolve_proph with "Hp").
+    iIntros (pvs') "[-> Hp]". simpl in Hpvs.
+    rewrite bool_decide_true in Hpvs; last done.
+    simpl in Hpvs.
+    iMod ("Hclose" with "[Hp]") as "HΦ".
+    { iExists (decode_actions pvs').
+      rewrite Hts in Hpvs. iSplit; first done.
+      iExists _. by iFrame. }
+    iModIntro. by iApply "HΦ".
+  Qed.
 
   Lemma wp_ResolveAbort p (tid : u64) (ts : nat) :
     ⊢
@@ -20,7 +33,21 @@ Section proph.
       ResolveAbort #p #tid @ ∅
     <<< ∃ acs', ⌜acs = ActAbort ts :: acs'⌝ ∗ own_txn_proph p acs' >>>
     {{{ RET #(); True }}}.
-  Admitted.
+  Proof.
+    iIntros "!> %Φ %Hts AU". wp_rec. wp_pures.
+    replace (⊤ ∖ ∅) with (⊤ : coPset) by set_solver.
+    iMod "AU" as (acs) "[(%pvs & %Hpvs & Hp) Hclose]".
+    wp_apply (wp_resolve_proph with "Hp").
+    iIntros (pvs') "[-> Hp]". simpl in Hpvs.
+    rewrite bool_decide_false in Hpvs; last done.
+    rewrite bool_decide_true in Hpvs; last done.
+    simpl in Hpvs.
+    iMod ("Hclose" with "[Hp]") as "HΦ".
+    { iExists (decode_actions pvs').
+      rewrite Hts in Hpvs. iSplit; first done.
+      iExists _. by iFrame. }
+    iModIntro. by iApply "HΦ".
+  Qed.
 
   Lemma wp_ResolveCommit
     p (tid : u64) (ts : nat) (wrsP : loc) q (wrs : dbmap) :
@@ -30,6 +57,29 @@ Section proph.
       ResolveCommit #p #tid #wrsP @ ∅
     <<< ∃ acs', ⌜acs = ActCommit ts wrs :: acs'⌝ ∗ own_txn_proph p acs' >>>
     {{{ RET #(); own_map wrsP q wrs }}}.
+  Proof.
+    iIntros "!> %Φ [%Hts Hm] AU". wp_rec. wp_pures.
+    replace (⊤ ∖ ∅) with (⊤ : coPset) by set_solver.
+    wp_rec.
+    rewrite /own_map /map.own_map.
+    iDestruct "Hm" as (mv ?) "Hmref".
+    wp_untyped_load. wp_pures.
+    iMod "AU" as (acs) "[(%pvs & %Hpvs & Hp) Hclose]".
+    wp_apply (wp_resolve_proph with "Hp").
+    iIntros (pvs') "[-> Hp]". simpl in Hpvs.
+    rewrite bool_decide_false in Hpvs; last done.
+    rewrite bool_decide_false in Hpvs; last done.
+    rewrite bool_decide_true in Hpvs; last done.
+    simpl in Hpvs.
+    iMod ("Hclose" with "[Hp]") as "HΦ".
+    { iExists (decode_actions pvs').
+      rewrite Hts in Hpvs.
+      iSplit.
+      { admit. (* todo: bad definition of decode dbmap *) }
+      iExists _. by iFrame. }
+    iModIntro. iApply "HΦ".
+    iFrame "Hmref".
+    eauto.
   Admitted.
 
 End proph.
